Fifteen/Logic/Basic.lean
@@ -13,4 +13,24 @@ theorem decide_or {p q : Prop} [Decidable p] [Decidable q] : decide (p ∨ q) = 
 theorem decide_and {p q : Prop} [Decidable p] [Decidable q] : decide (p ∧ q) = (decide p && decide q) := by
   apply dite p <;> apply dite q <;> intro hp hq <;> simp [hp, hq]
 
+theorem Bool.bne_comm (a b : Bool) : (a != b) = (b != a) := by
+  cases a <;> cases b <;> decide
+
+theorem Bool.bne_assoc (a b c : Bool) : ((a != b) != c) = (a != (b != c)) := by
+  cases a <;> cases b <;> cases c <;> decide
+
+@[simp]
+theorem Bool.bne_self (a : Bool) : (a != a) = false := by
+  cases a <;> decide
+
+@[simp]
+theorem Bool.bne_false (a : Bool) : (a != false) = a := by
+  cases a <;> decide
+
+@[simp]
+theorem Bool.false_bne (a : Bool) : (false != a) = a := by
+  cases a <;> decide
+
+theorem Bool.bne_eq_false (a b : Bool) : (a != b) = false ↔ a = b := by
+  cases a <;> cases b <;> decide
 
